lakefile.lean
@@ -1,16 +1,11 @@
 import Lake
 open Lake DSL
 
-package «interpolation» where
-  -- add package configuration options here
+package «fp-lab»
 
 lean_lib «Interpolation» where
-  -- add library configuration options here
+  roots := #[`Interpolation]
 
 @[default_target]
 lean_exe «interpolation» where
   root := `Main
-  -- Enables the use of the Lean interpreter by the executable (e.g.,
-  -- `runFrontend`) at the expense of increased binary size on Linux.
-  -- Remove this line if you do not need such functionality.
-  supportInterpreter := true
